LtlFrp/Structures.lean
@@ -1,0 +1,47 @@
+import LtlFrp.LTL
+
+namespace Monad
+-- ANCHOR: monad
+class Monad (m : Type → Type) where
+  -- The operations that a monad supports...
+  pure : α → m α -- Inject a value into the computational context
+  bind : m α → (α → m β) → m β -- Sequence a computation
+
+  -- ...and proofs of the monads laws
+  lid: bind (pure a) f = f a
+  rid : bind ma pure = ma
+  assoc : bind (bind ma f) g = bind ma (fun a => bind (f a) g)
+-- ANCHOR_END: monad
+
+-- ANCHOR: monad_ex
+inductive Perhaps α where
+  | nothing : Perhaps α
+  | indeed (a : α) : Perhaps α
+
+instance : Monad Perhaps where
+  pure a := Perhaps.indeed a
+  bind per f := match per with
+    | Perhaps.nothing => Perhaps.nothing
+    | Perhaps.indeed a => f a
+
+  lid := by simp
+  rid := by intros x ma; cases ma <;> rfl
+  assoc := by intros x ma; cases ma <;> simp
+-- ANCHOR_END: monad_ex
+
+end Monad
+
+-- ANCHOR: comonad
+class Comonad (w : Type → Type) where
+  extract : w α → α
+  extend  : w α → (w α → β) → w β
+
+  lid: extract (extend wa f) = f wa
+  rid: extend wa extract = wa
+  assoc: extend (extend wa f) g = extend wa (fun wa' => g (extend wa' f))
+-- ANCHOR_END: comonad
+
+
+namespace Examples
+
+end Examples
